theories/link.v
@@ -1,0 +1,245 @@
+Require Export refframe.module.
+Require Import refframe.trefines.
+Require Import refframe.filter.
+Require Import refframe.product.
+Require Import refframe.seq_product.
+Require Import refframe.proof_techniques.
+Require Import refframe.state_transform.
+
+Set Default Proof Using "Type".
+
+Section mod_link.
+  Context {EV : Type} {S : Type}.
+  Implicit Types (R : seq_product_state → S → EV → seq_product_state → S → EV → Prop).
+  Implicit Types (m : module (io_event EV)).
+
+  Inductive mod_link_state :=
+  | MLFLeft | MLFRight | MLFNone
+  | MLFRecvL (e : EV) | MLFRecvR (e : EV).
+
+  Definition mod_link_to_state (s : seq_product_state) (e : EV) : mod_link_state :=
+    match s with
+    | SPNone => MLFNone
+    | SPLeft => MLFRecvL e
+    | SPRight => MLFRecvR e
+    end.
+  Inductive mod_link_filter R : mod_map_fn (seq_product_event (io_event EV) (io_event EV)) (io_event EV) (mod_link_state * S) :=
+  | MLFLeftS s e p' s' e':
+    R SPLeft s e p' s' e' →
+    mod_link_filter R (MLFLeft, s) (SPELeft (Outgoing, e) p')
+                    (if p' is SPNone then Some (Outgoing, e') else None)
+                    (mod_link_to_state p' e', s')
+  | MLFLeftRecvS s e:
+    mod_link_filter R (MLFRecvL e, s) (SPELeft (Incoming, e) SPLeft) None (MLFLeft, s)
+  | MLFRightS s e p' s' e':
+    R SPRight s e p' s' e' →
+    mod_link_filter R (MLFRight, s) (SPERight (Outgoing, e) p')
+                    (if p' is SPNone then Some (Outgoing, e') else None)
+                    (mod_link_to_state p' e', s')
+  | MLFRightRecvS s e:
+    mod_link_filter R (MLFRecvR e, s) (SPERight (Incoming, e) SPRight) None (MLFRight, s)
+  | MLFNoneS s e p' s' e':
+    R SPNone s e p' s' e' →
+    mod_link_filter R (MLFNone, s) (SPENone p')
+                    (Some (Incoming, e'))
+                    (mod_link_to_state p' e', s')
+  .
+
+  Definition mod_link_trans R m1 m2 (σ : mod_link_state * S * m1.(m_state) * m2.(m_state)) :=
+    (match σ.1.1.1 with
+          | MLFLeft | MLFRecvL _ => SPLeft
+          | MLFRight | MLFRecvR _ => SPRight
+          | MLFNone => SPNone
+          end, σ.1.2, σ.2, σ.1.1).
+  Arguments mod_link_trans _ _ _ _ /.
+
+  Definition mod_link R m1 m2 : module (io_event EV) :=
+    mod_state_transform (mod_map (mod_seq_product m1 m2) (mod_link_filter R))
+                        (λ σ σ', σ' = mod_link_trans R m1 m2 σ).
+
+  Lemma mod_link_trefines R m1 m2 m1' m2' σ1 σ2 σ1' σ2' σ `{!VisNoAll m1} `{!VisNoAll m2}:
+    trefines (MS m1 σ1) (MS m1' σ1') →
+    trefines (MS m2 σ2) (MS m2' σ2') →
+    trefines (MS (mod_link R m1 m2) (σ, σ1, σ2)) (MS (mod_link R m1' m2') (σ, σ1', σ2')).
+  Proof.
+    move => ??.
+    apply: mod_state_transform_trefines; [| | |done..].
+    - move => [[??]?] [[[??]?]?] [[[??]?]?] /=. naive_solver.
+    - move => [[??]?] [[[??]?][??]] [[[??]?][??]] ?????; simplify_eq.
+      invert_all @m_step; invert_all @mod_link_filter; destruct_all?; simplify_eq.
+      all: eexists (_, _, _); do 3 f_equal; repeat case_match => //; simplify_eq/= => //.
+      all: unfold mod_link_to_state in *; by repeat case_match.
+    - apply mod_map_trefines => /=. by apply mod_seq_product_trefines.
+  Qed.
+
+  Lemma mod_link_step_left_i R m1 m2 s σ1 σ2 P `{!TStepI m1 σ1 P} :
+    TStepI (mod_link R m1 m2) (MLFLeft, s, σ1, σ2) (λ G, P (λ b κ P',
+      match κ with
+      | None => G b None (λ G', P' (λ x, G' (MLFLeft, s, x, σ2)))
+      | Some (Outgoing, e) => ∀ p' s' e', R SPLeft s e p' s' e' →
+                              G b (if p' is SPNone then Some (Outgoing, e') else None)
+                               (λ G', P' (λ x, G' (mod_link_to_state p' e', s', x, σ2)))
+      | Some _ => True
+      end)).
+  Proof.
+    constructor => G /tstepi_proof?. clear TStepI0.
+    apply: (steps_impl_submodule _ (mod_link _ _ _) (λ x, (MLFLeft, s, x, σ2))); [done| |].
+    - naive_solver.
+    - move => /= ??? Hs. invert_all' @state_transform_step; simplify_eq. invert_all' @m_step; simplify_eq/=.
+      + case_match; simplify_eq. naive_solver.
+      + case_match; simplify_eq. invert_all @mod_link_filter.
+        split!; [done| |done] => /=?. destruct_all?.
+        split!; [naive_solver..|]. move => /= ? HP. move: HP => /H2[?[??]]. eexists (_, _, _, _).
+        split!; [|naive_solver] => /=. by destruct s0.
+  Qed.
+
+  Lemma mod_link_step_right_i R m1 m2 s σ1 σ2 P `{!TStepI m2 σ2 P} :
+    TStepI (mod_link R m1 m2) (MLFRight, s, σ1, σ2) (λ G, P (λ b κ P',
+      match κ with
+      | None => G b None (λ G', P' (λ x, G' (MLFRight, s, σ1, x)))
+      | Some (Outgoing, e) => ∀ p' s' e', R SPRight s e p' s' e' →
+                              G b (if p' is SPNone then Some (Outgoing, e') else None)
+                               (λ G', P' (λ x, G' (mod_link_to_state p' e', s', σ1, x)))
+      | Some _ => True
+      end)).
+  Proof.
+    constructor => G /tstepi_proof?. clear TStepI0.
+    apply: (steps_impl_submodule _ (mod_link _ _ _) (λ x, (MLFRight, s, σ1, x))); [done| |].
+    - naive_solver.
+    - move => /= ??? Hs. invert_all' @state_transform_step; simplify_eq. invert_all' @m_step; simplify_eq/=.
+      + case_match; simplify_eq. naive_solver.
+      + case_match; simplify_eq. invert_all @mod_link_filter.
+        split!; [done| |done] => /=?. destruct_all?.
+        split!; [naive_solver..|]. move => /= ? HP. move: HP => /H2[?[??]]. eexists (_, _, _, _).
+        split!; [|naive_solver] => /=. by destruct s0.
+  Qed.
+
+  Lemma mod_link_step_left_recv_i R m1 m2 s σ1 σ2 e P `{!TStepI m1 σ1 P} :
+    TStepI (mod_link R m1 m2) (MLFRecvL e, s, σ1, σ2) (λ G, P (λ b κ P',
+      match κ with
+      | None => G b None (λ G', P' (λ x, G' (MLFRecvL e, s, x, σ2)))
+      | Some (Incoming, e') => e = e' → G b None (λ G', P' (λ x, G' (MLFLeft, s, x, σ2)))
+      | Some _ => True
+      end)).
+  Proof.
+    constructor => G /tstepi_proof?. clear TStepI0.
+    apply: (steps_impl_submodule _ (mod_link _ _ _) (λ x, (MLFRecvL e, s, x, σ2))); [done| |].
+    - naive_solver.
+    - move => /= ??? Hs. invert_all' @state_transform_step; simplify_eq. invert_all' @m_step; simplify_eq/=.
+      + case_match; simplify_eq. naive_solver.
+      + case_match; simplify_eq. invert_all @mod_link_filter; naive_solver.
+  Qed.
+
+  Lemma mod_link_step_right_recv_i R m1 m2 s σ1 σ2 e P `{!TStepI m2 σ2 P} :
+    TStepI (mod_link R m1 m2) (MLFRecvR e, s, σ1, σ2) (λ G, P (λ b κ P',
+      match κ with
+      | None => G b None (λ G', P' (λ x, G' (MLFRecvR e, s, σ1, x)))
+      | Some (Incoming, e') => e = e' → G b None (λ G', P' (λ x, G' (MLFRight, s, σ1, x)))
+      | Some _ => True
+      end)).
+  Proof.
+    constructor => G /tstepi_proof?. clear TStepI0.
+    apply: (steps_impl_submodule _ (mod_link _ _ _) (λ x, (MLFRecvR e, s, σ1, x))); [done| |].
+    - naive_solver.
+    - move => /= ??? Hs. invert_all' @state_transform_step; simplify_eq. invert_all' @m_step; simplify_eq/=.
+      + case_match; simplify_eq. naive_solver.
+      + case_match; simplify_eq. invert_all @mod_link_filter; naive_solver.
+  Qed.
+
+  Lemma mod_link_step_none_i R m1 m2 s σ1 σ2 :
+    TStepI (mod_link R m1 m2) (MLFNone, s, σ1, σ2) (λ G, ∀ e p' s' e', R SPNone s e p' s' e' →
+      G true (Some (Incoming, e')) (λ G', G' (mod_link_to_state p' e', s', σ1, σ2))).
+  Proof.
+    constructor => G HG. apply steps_impl_step_end => ???.
+    invert_all' @m_step; simplify_eq/=; invert_all' mod_link_filter; simplify_eq/=.
+    split!; [naive_solver|done|] => /= ??. eexists (_, _, _, _). split!; [|done] => /=. by destruct s0.
+  Qed.
+
+  Lemma mod_link_step_left_s R m1 m2 s σ1 σ2 P `{!TStepS m1 σ1 P} :
+    TStepS (mod_link R m1 m2) (MLFLeft, s, σ1, σ2) (λ G, P (λ κ P',
+      match κ with
+      | None => G None (λ G', P' (λ x, G' (MLFLeft, s, x, σ2)))
+      | Some (Outgoing, e) => ∃ p' s' e', R SPLeft s e p' s' e' ∧
+                              G (if p' is SPNone then Some (Outgoing, e') else None)
+                               (λ G', P' (λ σ', G' (mod_link_to_state p' e', s', σ', σ2)))
+      | Some _ => False
+      end)).
+  Proof.
+    constructor => G /tsteps_proof [κ [? [? HG']]]. clear TStepS0.
+    destruct κ as [[[] e]|] => //; destruct_all?.
+    all: eexists _, _; split; [done|] => G' /= /HG'?; tstep_s.
+    all: split!; [..|apply: steps_spec_mono; [done|]] => //=; try by econs.
+    all: move => ?? [[[p?]?]?]//=?; destruct p => //; by simplify_eq/=.
+  Qed.
+
+  Lemma mod_link_step_right_s R m1 m2 s σ1 σ2 P `{!TStepS m2 σ2 P} :
+    TStepS (mod_link R m1 m2) (MLFRight, s, σ1, σ2) (λ G, P (λ κ P',
+      match κ with
+      | None => G None (λ G', P' (λ x, G' (MLFRight, s, σ1, x)))
+      | Some (Outgoing, e) => ∃ p' s' e', R SPRight s e p' s' e' ∧
+                              G (if p' is SPNone then Some (Outgoing, e') else None)
+                               (λ G', P' (λ σ', G' (mod_link_to_state p' e', s', σ1, σ')))
+      | Some _ => False
+      end)).
+  Proof.
+    constructor => G /tsteps_proof [κ [? [? HG']]]. clear TStepS0.
+    destruct κ as [[[] e]|] => //; destruct_all?.
+    all: eexists _, _; split; [done|] => G' /= /HG'?; tstep_s.
+    all: split!; [..|apply: steps_spec_mono; [done|]] => //=; try by econs.
+    all: move => ?? [[[p?]?]?]//=?; destruct p => //; by simplify_eq/=.
+  Qed.
+
+  Lemma mod_link_step_left_recv_s R m1 m2 s σ1 σ2 e P `{!TStepS m1 σ1 P} :
+    TStepS (mod_link R m1 m2) (MLFRecvL e, s, σ1, σ2) (λ G, P (λ κ P',
+      match κ with
+      | None => G None (λ G', P' (λ x, G' (MLFRecvL e, s, x, σ2)))
+      | Some (Incoming, e') => G None (λ G', e = e' ∧ P' (λ x, G' (MLFLeft, s, x, σ2)))
+      | Some _ => False
+      end)).
+  Proof.
+    constructor => G /tsteps_proof [κ [? [? HG']]]. clear TStepS0.
+    destruct κ as [[[] e']|] => //; destruct_all?.
+    all: eexists _, _; split; [done|] => G' /=; try move => [?]; move => /HG'?; tstep_s; simplify_eq.
+    all: split!; [..|apply: steps_spec_mono; [done|]] => //=; try by econs.
+    all: move => ?? [[[p?]?]?]//=?; destruct p => //; by simplify_eq/=.
+  Qed.
+
+  Lemma mod_link_step_right_recv_s R m1 m2 s σ1 σ2 e P `{!TStepS m2 σ2 P} :
+    TStepS (mod_link R m1 m2) (MLFRecvR e, s, σ1, σ2) (λ G, P (λ κ P',
+      match κ with
+      | None => G None (λ G', P' (λ x, G' (MLFRecvR e, s, σ1, x)))
+      | Some (Incoming, e') => G None (λ G', e = e' ∧ P' (λ x, G' (MLFRight, s, σ1, x)))
+      | Some _ => False
+      end)).
+  Proof.
+    constructor => G /tsteps_proof [κ [? [? HG']]]. clear TStepS0.
+    destruct κ as [[[] e']|] => //; destruct_all?.
+    all: eexists _, _; split; [done|] => G' /=; try move => [?]; move => /HG'?; tstep_s; simplify_eq.
+    all: split!; [..|apply: steps_spec_mono; [done|]] => //=; try by econs.
+    all: move => ?? [[[p?]?]?]//=?; destruct p => //; by simplify_eq/=.
+  Qed.
+
+  Lemma mod_link_step_none_s R m1 m2 s σ1 σ2 :
+    TStepS (mod_link R m1 m2) (MLFNone, s, σ1, σ2) (λ G, ∃ e p' s' e', R SPNone s e p' s' e' ∧
+      G (Some (Incoming, e')) (λ G', G' (mod_link_to_state p' e', s', σ1, σ2))).
+  Proof.
+    constructor => G [?[?[?[?[??]]]]]. split!; [done|] => /=??.
+    tstep_s. split!; [by econs|]. move => [[[??]?]?] /=. unfold mod_link_to_state.
+    repeat case_match; naive_solver.
+  Qed.
+End mod_link.
+Arguments mod_link_trans _ _ _ _ _ /.
+Arguments mod_link_state : clear implicits.
+
+Global Hint Resolve
+       mod_link_step_left_i
+       mod_link_step_right_i
+       mod_link_step_left_recv_i
+       mod_link_step_right_recv_i
+       mod_link_step_none_i
+       mod_link_step_left_s
+       mod_link_step_right_s
+       mod_link_step_left_recv_s
+       mod_link_step_right_recv_s
+       mod_link_step_none_s
+| 2 : tstep.
